Protocol/httpprotocol.fst
@@ -1,6 +1,0 @@
-module HttpProtocol
-
-type HttpMessage =
-  | Get: uri -> HttpMessage
-  | Post: uri -> HttpMessage
-  | Redirect: destination -> message -> HttpMessage
