Protocol/identityprovider.fst
@@ -44,9 +44,9 @@ let rec identityprovider me client =
         identityprovider me client (*Start over*)
       )
     else
-      SendSaml client (DisplayError 400);(*8.1*)
+      SendSaml client (DisplayError 400);(*10.1*)
       identityprovider me client (*Start over*)
 
-  | _ -> SendSaml client (DisplayError 400);(*8.1*)
+  | _ -> SendSaml client (DisplayError 400);(*10.1*)
         identityprovider me client (*Start over*)
 
