Protocol/main.fst
@@ -8,8 +8,6 @@ open Identityprovider
 val Fork: list (unit -> unit) -> unit
 
 let main attacker =
-	let sppk, spsk = Keygen "https://serviceprovider.org" in 
-	let idppk, idpsk = Keygen "https://identityprovider.org" in 
 	Fork [	attacker;
-		(fun () -> serviceprovider "https://serviceprovider.org" "browser" "https://identityprovider.org");
-		(fun () -> identityprovider "https://identityprovider.org" "browser")]
+		(fun () -> serviceprovider "serviceprovider.org" "browser" "identityprovider.org");
+		(fun () -> identityprovider "identityprovider.org" "browser")]
