Protocol/samltypes.fst
@@ -1,6 +1,0 @@
-module samltypes
-
-type AuthnRequest = {id:string;  
-                    IssueInstant:string;     
-                    Destination:endpoint;
-                    Issuer:prin}
